Add option -fno-tailcalls to turn off tailcall elimination (causes problem with some static analysis tools). */PrintAsm.ml: don't cfa_adjust at Pfreeframe, as more code from the function can appear after (in case of tailcalls).
git-svn-id: https://yquem.inria.fr/compcert/svn/compcert/trunk@2256 fca1b0fc-160b-0410-b1d3-a4f43f01ea2e

arm/PrintAsm.ml
@@ -648,9 +648,7 @@ let print_instruction oc = function
   | Pfreeframe(sz, ofs) ->
       if Asmgen.is_immed_arith sz
       then fprintf oc "	add	sp, sp, #%a\n" coqint sz
-      else fprintf oc "	ldr	sp, [sp, #%a]\n" coqint ofs;
-      cfi_adjust oc (Int32.neg (camlint_of_coqint sz));
-      1
+      else fprintf oc "	ldr	sp, [sp, #%a]\n" coqint ofs; 1
   | Plabel lbl ->
       fprintf oc "%a:\n" print_label lbl; 0
   | Ploadsymbol(r1, id, ofs) ->
