driver/Clflags.ml
@@ -22,6 +22,7 @@ let option_fvararg_calls = ref true
 let option_fpacked_structs = ref false
 let option_fsse = ref true
 let option_ffloatconstprop = ref 2
+let option_ftailcalls = ref true
 let option_falignfunctions = ref (None: int option)
 let option_falignbranchtargets = ref 0
 let option_faligncondbranchs = ref 0
